rust/implementation/openssl3_impl/tunnel/mod.rs
@@ -4,14 +4,52 @@
 //! Tunnel implementation using OpenSSL 3 and oqs-provider.
 
 use bio_method::BIO_METHOD;
-pub use context::Context;
-pub(crate) use ssl::Tunnel;
 use ssl::{Ssl, TunnelBuilder};
 use verify_callback::verify_callback;
 use x509_verify_param::X509VerifyParam;
+use crate::support::Pimpl;
+use crate::ossl3::NativeSsl;
+use crate::ossl3::NativeSslCtx;
+use crate::tunnel::tls;
+use crate::tunnel::BoxedIO;
+use crate::tunnel::Mode;
+use crate::ossl3::LibCtx;
 
 mod bio_method;
 mod context;
 mod ssl;
 mod verify_callback;
 mod x509_verify_param;
+
+/// A tunnel, wrapper around a SSL object.
+pub struct Tunnel<'a> {
+    /// Parent SSL_CTX object.
+    pub(crate) _ssl_ctx: &'a Context<'a>,
+
+    /// SSL object.
+    pub(crate) ssl: Pimpl<'a, NativeSsl>,
+
+    /// Security requirements from the verifiers.
+    pub(crate) security_requirements: tls::TunnelSecurityRequirements,
+
+    /// IO interface.
+    pub(crate) io: BoxedIO,
+
+    /// state.
+    pub(crate) state: pb::State,
+}
+
+/// Tunnel context.
+pub struct Context<'a> {
+    /// Library context parent.
+    _lib_ctx: &'a LibCtx<'a>,
+
+    /// `SSL_CTX` object.
+    ssl_ctx: Pimpl<'a, NativeSslCtx>,
+
+    /// Security requirements from the verifiers.
+    security_requirements: tls::TunnelSecurityRequirements,
+
+    /// Execution mode.
+    mode: Mode,
+}
