proofs/fstar/extraction/Sandwich.Implementation.Openssl3_impl.Tunnel.fsti
@@ -1,0 +1,21 @@
+module Sandwich.Implementation.Openssl3_impl.Tunnel
+#set-options "--fuel 0 --ifuel 1 --z3rlimit 15"
+open Core
+open FStar.Mul
+
+/// Tunnel context.
+type t_Context = {
+  f__lib_ctx:Sandwich.Implementation.Openssl3_impl.t_LibCtx;
+  f_ssl_ctx:Sandwich.Support.Pimpl.t_Pimpl Openssl3.t_ssl_ctx_st;
+  f_security_requirements:Sandwich.Tunnel.Tls.t_TunnelSecurityRequirements;
+  f_mode:Sandwich.Tunnel.Context.t_Mode
+}
+
+/// A tunnel, wrapper around a SSL object.
+type t_Tunnel = {
+  f__ssl_ctx:t_Context;
+  f_ssl:Sandwich.Support.Pimpl.t_Pimpl Openssl3.t_ssl_st;
+  f_security_requirements:Sandwich.Tunnel.Tls.t_TunnelSecurityRequirements;
+  f_io:Sandwich.Tunnel.Io.t_BoxedIO;
+  f_state:Sandwich_proto.Tunnel.t_State
+}
